fix up proof

examples/lambda/Lambda.hs
@@ -8,23 +8,24 @@ data Expr
   | Lam Name Expr
   | App Expr Expr
 
-
+-- Data.Foldable.maximum is a partial function (fails when the list is empty)
+-- So we use a total version that requires a nonempty list.
 maxName :: Name -> [Name] -> Name
 maxName n ns = foldr max n ns
 
 maxVar :: Expr -> Int
-maxVar (Var n) = n
+maxVar (Var n)       = n
 maxVar (Let n e1 e2) = maxName n [maxVar e1, maxVar e2]
-maxVar (Lam n e) = maxName  n [maxVar e]
-maxVar (App e1 e2) = maxName (maxVar e1) [maxVar e2]
+maxVar (Lam n e)     = maxName  n [maxVar e]
+maxVar (App e1 e2)   = maxName (maxVar e1) [maxVar e2]
 
 fresh :: Expr -> Int
 fresh e = 1 + maxVar e
 
 anf :: Expr -> Expr
-anf (Var n) = Var n
+anf (Var n)          = Var n
 anf (Let n rhs body) = Let n (anf rhs) (anf body)
-anf (Lam n body) = Lam n (anf body)
-anf (App f (Var n)) = App (anf f) (Var n)
-anf (App f e) = Let v (anf e) (App (anf f) (Var v))
+anf (Lam n body)     = Lam n (anf body)
+anf (App f (Var n))  = App (anf f) (Var n)
+anf (App f e)        = Let v (anf e) (App (anf f) (Var v))
   where v = fresh f
